Bloom filter updates

theories/coneris/examples/bloom_filter/bloom_filter.v
@@ -1,4 +1,5 @@
 From iris.base_logic.lib Require Import invariants.
+From iris.algebra Require Import gset_bij.
 From clutch.coneris Require Import coneris par spawn spin_lock hash atomic lock concurrent_hash.
 From clutch.coneris.lib Require Import list array.
 
@@ -8,11 +9,13 @@ Section bloom_filter.
 
   Variable filter_size : nat.
   Variable num_hash : nat.
-  Variable insert_num : nat.
-  Variable max_hash_size : nat.
-  Hypothesis max_hash_size_pos: (0<max_hash_size)%nat.
+  (* Variable insert_num : nat. *)
+  (* Variable max_hash_size : nat.*)
+  (* Hypothesis max_hash_size_pos: (0<max_hash_size)%nat. *)
 
-  Context `{!conerisGS Σ}.
+  Context `{!conerisGS Σ, HinG: inG Σ (gset_bijR nat nat)}.
+
+  Search nonnegreal.
 
   Fixpoint fp_error (m l b : nat) : R :=
       (match m with
@@ -47,6 +50,10 @@ Section bloom_filter.
     destruct m; done.
   Qed.
 
+  Lemma fp_error_weaken (m l b : nat) :
+    (fp_error 0 0 b <= fp_error m l b)%R.
+  Admitted.
+
   Lemma fp_error_nonneg (m l b : nat) :
     (0 <= fp_error m l b)%R.
   Admitted.
@@ -55,194 +62,492 @@ Section bloom_filter.
 
   Definition init_bloom_filter : expr :=
     λ: "_" ,
-      let: "h1" := init_hash filter_size #() in
-      let: "h2" := init_hash filter_size #() in
+      let: "hfuns" := list_seq_fun #0 #num_hash (λ: "_", init_hash filter_size #())%E in
       let: "arr" := array_init #(S filter_size) (λ: "x", #false)%E in
-      let: "l" := ref ("h1", "h2", "arr") in
+      let: "l" := ref ("hfuns", "arr") in
       "l".
 
   Definition insert_bloom_filter : expr :=
     λ: "l" "v" ,
-      let, ("h1", "h2", "arr") := !"l" in
-      let: "i1" := "h1" "v" in
-      let: "i2" := "h2" "v" in
-      "arr" +ₗ "i1" <- #true ;;
-      "arr" +ₗ "i2" <- #true ;;
-      #().
+      let, ("hfuns", "arr") := !"l" in
+      list_iter (λ: "h",
+          let: "i" := "h" "v" in
+          "arr" +ₗ "i" <- #true) "hfuns".
 
 
+  Definition lookup_bloom_filter : expr :=
+    λ: "l" "v" ,
+      let, ("hfuns", "arr") := !"l" in
+      let: "res" := ref #true in
+      list_iter (λ: "h",
+          let: "i" := "h" "v" in
+          if: !("arr" +ₗ "i") then #() else "res" <- #false) "hfuns";;
+      !"res".
 
-  Definition is_bloom_filter (l : loc) (els : gset nat) (bs : nat) : iProp Σ :=
-    ∃ h1 h2 m1 m2 a arr (idxs : gset nat),
-      l ↦ (h1, h2, LitV (LitLoc a))%V ∗
-        hashfun filter_size h1 m1 ∗ hashfun filter_size h2 m2 ∗
+
+  Definition is_bloom_filter (l : loc) (els : gset nat) (rem : nat) : iProp Σ :=
+    ∃ hfuns hs ms a arr (idxs : gset nat),
+      ↯ (fp_error rem 0 (size idxs)) ∗
+      l ↦ (hfuns, LitV (LitLoc a))%V ∗
+        ⌜ is_list_HO hs hfuns ⌝ ∗
+        ⌜ length hs = num_hash ⌝ ∗
+        ([∗ list] k↦h;m ∈ hs;ms, hashfun filter_size h m) ∗
         ⌜ length arr = S filter_size ⌝ ∗
         (a ↦∗ arr) ∗
-        ⌜ els = dom m1 ⌝ ∗ ⌜ els = dom m2 ⌝ ∗
-        ⌜ forall e, e ∈ els -> (m1 !!! e) ∈ idxs  ⌝ ∗
-        ⌜ forall e, e ∈ els -> (m2 !!! e) ∈ idxs  ⌝ ∗
+        ⌜ Forall (λ m, els = dom m) ms ⌝ ∗
+        ⌜ forall e, e ∈ els -> Forall (λ m, (m !!! e) ∈ idxs ) ms ⌝ ∗
         ⌜ forall i, i ∈ idxs -> arr !! i = Some #true  ⌝ ∗
         ⌜ forall i, i ∈ idxs -> (i < S filter_size)%nat  ⌝ ∗
-        ⌜ forall i, i < S filter_size -> i ∉ idxs -> arr !! i = Some #false  ⌝ ∗
-        ⌜ bs = size idxs ⌝.
+        ⌜ forall i, i < S filter_size -> i ∉ idxs -> arr !! i = Some #false  ⌝.
 
 
+  Definition is_bloom_filter_partial (l : loc) (e_new : nat)
+    (els : gset nat) (rem : nat) hs_new hs_old a : iProp Σ :=
+    ∃ hfuns ms_new ms_old arr (idxs : gset nat),
+      ↯ (fp_error rem (length hs_old) (size idxs)) ∗
+      l ↦ (hfuns, LitV (LitLoc a))%V ∗
+        ⌜ is_list_HO (hs_new ++ hs_old) hfuns ⌝ ∗
+        ⌜ length (hs_new ++ hs_old) = num_hash ⌝ ∗
+        ([∗ list] k↦h;m ∈ hs_new;ms_new, hashfun filter_size h m) ∗
+        ([∗ list] k↦h;m ∈ hs_old;ms_old, hashfun filter_size h m) ∗
+        ⌜ length arr = S filter_size ⌝ ∗
+        (a ↦∗ arr) ∗
+        ⌜ Forall (λ m, els = dom m) ms_old ⌝ ∗
+        ⌜ Forall (λ m, ({[e_new]} ∪ els) = dom m) ms_new ⌝ ∗
+        ⌜ forall e, e ∈ els -> Forall (λ m, (m !!! e) ∈ idxs ) ms_old ⌝ ∗
+        ⌜ forall e, e ∈ ({[e_new]} ∪ els) ->
+               Forall (λ m, (m !!! e) ∈ idxs ) ms_new ⌝ ∗
+        ⌜ forall i, i ∈ idxs -> arr !! i = Some #true  ⌝ ∗
+        ⌜ forall i, i ∈ idxs -> (i < S filter_size)%nat  ⌝ ∗
+        ⌜ forall i, i < S filter_size -> i ∉ idxs -> arr !! i = Some #false  ⌝.
 
-  Lemma bloom_filter_init_spec :
-    {{{ True }}}
-      init_bloom_filter #()
-      {{{ (l:loc), RET #l ; is_bloom_filter l ∅ 0 }}}.
+  Definition bloom_filter_to_partial l e_new els rem :
+    is_bloom_filter l els (S rem) -∗
+     ∃ hs a , is_bloom_filter_partial l e_new els rem [] hs a.
   Proof.
-    iIntros (Φ) "_ HΦ".
+    iIntros "Hbf".
+    iDestruct "Hbf" as (hfuns hs ms a arr idxs) "(Hl & Herr & %Hhfuns & %Hlenhs & Hhs & %HlenA & Ha & %Hms & %Hidxs & %Htrue & %Hbd & %Hfalse)".
+    rewrite fp_error_S_Z.
+    iExists hs, a.
+    rewrite /is_bloom_filter_partial.
+    iExists hfuns, [] , ms , arr, idxs.
+    simpl.
+    rewrite Hlenhs.
+    iFrame.
+    iPureIntro.
+    repeat split; auto.
+  Qed.
+
+  Definition bloom_filter_from_partial l e_new els hs a rem :
+    is_bloom_filter_partial l e_new els rem hs [] a -∗
+      is_bloom_filter l ({[e_new]} ∪ els) rem.
+  Proof.
+    iIntros "Hbfp".
+    iDestruct "Hbfp" as (hfuns ms_new ms_old arr idxs)
+                          "(Hl & Herr & %Hhfuns & %Hlenhs & Hhs_new & Hhs_old & %HlenA & Ha & %Hms_old & %Hms_new & %Hidxs_old & %Hidxs_new & %Htrue & %Hbd & %Hfalse)".
+    rewrite /is_bloom_filter.
+    iExists hfuns, hs, ms_new, a, arr, idxs.
+    iFrame.
+    iPureIntro.
+    rewrite app_nil_r in Hhfuns.
+    rewrite app_nil_r in Hlenhs.
+    repeat split; auto.
+  Qed.
+
+
+  Lemma bloom_filter_init_spec (rem : nat) :
+    {{{ ↯ (fp_error rem 0 0) }}}
+      init_bloom_filter #()
+      {{{ (l:loc), RET #l ; is_bloom_filter l ∅ rem }}}.
+  Proof using HinG conerisGS0 filter_size Σ.
+    iIntros (Φ) "Herr HΦ".
     rewrite /init_bloom_filter.
     wp_pures.
-    wp_apply (wp_init_hash); auto.
-    iIntros (h1) "(%γ1 & Hh1)".
-    wp_pures.
-    wp_apply (wp_init_hash); auto.
-    iIntros (h2) "(%γ2 & Hh2)".
-    wp_pures.
-    wp_apply (wp_array_init (λ _ v, ⌜ v = #false ⌝%I)).
-    - admit.
-    - iApply big_sepL_intro.
+    wp_bind (list_seq_fun _ _ _).
+    wp_apply (wp_list_seq_fun_HO _ 0 num_hash _
+                (λ _ v, hashfun filter_size v ∅)%I).
+    {
+      iIntros (i Φ').
       iModIntro.
-      iIntros (??) "?".
+      iIntros "_ HΦ".
       wp_pures.
-      done.
-    - iIntros (a arr) "(%Hlen & Ha & %Harr)".
+      wp_apply wp_init_hash_basic; auto.
+    }
+    - iIntros (v vs) "(%Hvs & %Hlen & Hg)".
       wp_pures.
-      wp_alloc l as "Hl".
-      wp_pures.
-      iMod "Hh1" as "(Hh1h & Hh1a)".
-      iMod "Hh2" as "(Hh2h & Hh2a)".
-      iModIntro.
-      iApply "HΦ".
-      rewrite /is_bloom_filter.
-      iExists h1, h2, ∅, ∅, a, arr, ∅.
-      iFrame.
-      iSplit.
-      {
+      wp_apply (wp_array_init (λ _ v, ⌜ v = #false ⌝%I)).
+      + real_solver.
+      + iApply big_sepL_intro.
+        iModIntro.
+        iIntros (??) "?".
+        wp_pures.
+        done.
+      + iIntros (a arr) "(%HlenA & Ha & %Harr)".
+        wp_pures.
+        wp_alloc l as "Hl".
+        wp_pures.
+        iModIntro.
+        iApply "HΦ".
+        rewrite /is_bloom_filter.
+        iExists v, vs, (repeat ∅ num_hash), a, arr, ∅.
+        rewrite size_empty.
+        iFrame.
+        iSplit.
+        {
+          iPureIntro.
+          set_solver.
+        }
+        iSplit; [done |].
+        iSplit.
+        {
+          iApply big_sepL2_alt.
+          iRevert "Hg".
+          iInduction num_hash as [|nh] "IH" forall (v vs Hvs Hlen); iIntros "Hg".
+          - destruct vs; auto.
+          - simpl.
+            destruct vs as [|v' vs']; auto.
+            iSplitR; auto.
+            + iPureIntro.
+              rewrite repeat_length //.
+            + simpl.
+              iDestruct "Hg" as "[? Hg]".
+              iFrame.
+              destruct Hvs as [v'' [? ?]].
+              iPoseProof ("IH" $! v'' vs' _ _ with "[Hg]") as "[? ?]"; auto.
+              Unshelve. all:auto.
+        }
         iPureIntro.
-        set_solver.
-      }
-      iSplit.
-      {
-        iPureIntro.
-        set_solver.
-      }
-      iPureIntro.
-      split; [set_solver |].
-      split; [set_solver |].
-      split; [set_solver |].
-      split; [set_solver |].
-      split; [set_solver |].
-      split; [|set_solver].
-      intros i ??.
-      apply Nat2Z.inj' in Hlen.
-      rewrite <- Hlen in H.
-      pose proof (lookup_lt_is_Some_2 arr i H) as [x Hx].
-      specialize (Harr i x Hx).
-      rewrite Hx Harr //.
-  Admitted.
+        repeat split.
+        * set_solver.
+        * revert v vs Hvs Hlen.
+          induction num_hash; intros v vs Hvs Hlen.
+          ** simpl.
+             by apply Forall_nil.
+          ** simpl.
+             destruct vs; [inversion Hlen | ].
+             destruct Hvs as [? [? ?]].
+             apply Forall_cons; split; auto.
+             eapply IHn; eauto.
+        * set_solver.
+        * set_solver.
+        * set_solver.
+        * intros i H ?.
+          apply Nat2Z.inj' in HlenA.
+          rewrite <- HlenA in H.
+          pose proof (lookup_lt_is_Some_2 arr i H) as [x Hx].
+          specialize (Harr i x Hx).
+          rewrite Hx Harr //.
+  Qed.
 
 
-  Lemma bloom_filter_insert_spec (l : loc) (s : gset nat) (bs x m c : nat) :
-    {{{ is_bloom_filter l s bs ∗ ⌜ x ∉ s ⌝ ∗
-         ↯ (fp_error m (S (S c)) bs)
+  Lemma bloom_filter_insert_spec (l : loc) (s : gset nat) (x rem : nat) :
+    {{{ is_bloom_filter l s (S rem) ∗ ⌜ x ∉ s ⌝
     }}}
       insert_bloom_filter #l #x
-      {{{ RET #() ;
-          ∃ (i: nat),
-            is_bloom_filter l (s ∪ {[x]}) (bs + i) ∗
-              ↯ (fp_error m c (bs + i))
+      {{{ RET #() ; is_bloom_filter l (s ∪ {[x]}) rem
       }}}.
   Proof.
-    iIntros (Φ) "(Hbf & %Hx & Herr) HΦ".
+    iIntros (Φ) "(Hbf & %Hx ) HΦ".
     rewrite /insert_bloom_filter /is_bloom_filter.
     wp_pures.
-    iDestruct "Hbf" as (h1 h2 m1 m2 a arr idxs) "(Hl & Hh1 & Hh2 & %HlenA & Ha & %Hm1 & %Hm2 & %Hidxs1 & %Hidxs2 & %Htrue & %Hbd & %Hfalse & %Hbs)".
+    iDestruct "Hbf" as (hfuns hs ms a arr idxs) "(Herr & Hl & %Hfuns & Hrest)".
     wp_load.
     wp_pures.
-    wp_bind (h1 _).
-    wp_apply (wp_insert_avoid_set_adv filter_size _ _ m1 _ idxs
-                (mknonnegreal (fp_error m (S (S c)) bs) (fp_error_nonneg m (S (S c)) bs))
-                (mknonnegreal (fp_error m (S c) bs) (fp_error_nonneg m (S c) bs))
-                (mknonnegreal (fp_error m (S c) (S bs)) (fp_error_nonneg m (S c) (S bs)))
-               with
-             "[$]").
-    - apply not_elem_of_dom_1.
-      set_solver.
-    - auto.
-    - simpl.
-      rewrite fp_error_m_S -Hbs /=.
-      lra.
-    - iIntros (v1) "(%Hv1 & Hh1 & [(%HOut1 & Herr)|(%HIn1 & Herr )])".
+    iAssert (is_bloom_filter_partial l x s rem [] hs a ) with "[Hl Herr Hrest]" as "Hbfp".
+    {
+      iExists hfuns, [] , ms , arr, idxs.
+      simpl.
+      iDestruct "Hrest" as "(<- & ? & -> & ? & % & % & % & % & %)".
+      iFrame.
+      iPureIntro.
+      repeat split; auto.
+    }
+    wp_apply (wp_list_iter_invariant_HO
+                (λ l1 l2, is_bloom_filter_partial l x s rem l1 l2 a )%I
+               with "[][$Hbfp][HΦ]"); auto.
+    - iIntros (lpre w lsuf Ψ).
+      iModIntro.
+      iIntros "Hbfp HK".
+      wp_pures.
+      iDestruct "Hbfp" as (hfuns' ms_new ms_old arr' idxs')
+             "(Hl & Herr & %Hhfuns & %Hlenhs & Hhs_new & Hhs_old & %HlenA & Ha & %Hms_old & %Hms_new & %Hidxs_old & %Hidxs_new & %Htrue & %Hbd & %Hfalse)".
+      destruct ms_old as [| mcur ms_old_tl]; [set_solver|].
+      simpl.
+      iDestruct "Hhs_old" as "(Hhs_cur & Hhs_rest)".
+      apply Forall_cons_1 in Hms_old as [??].
+      wp_apply (wp_insert_avoid_set_adv filter_size _ _ mcur _ idxs'
+         (mknonnegreal (fp_error rem (S (length lsuf)) (size idxs'))
+            (fp_error_nonneg rem (S (length lsuf)) (size idxs')))
+         (mknonnegreal (fp_error rem (length lsuf) (size idxs'))
+            (fp_error_nonneg rem (length lsuf) (size idxs')))
+         (mknonnegreal (fp_error rem (length lsuf) (S (size idxs')))
+            (fp_error_nonneg rem (length lsuf) (S (size idxs')))) with "[$]").
+      + apply not_elem_of_dom_1.
+        set_solver.
+      + auto.
       + simpl.
-        wp_pures.
-        wp_bind (h2 _).
-        wp_apply (wp_insert_avoid_set_adv filter_size _ _ m2 _ (idxs ∪ {[v1]})
-                    (mknonnegreal (fp_error m (S c) (S bs)) (fp_error_nonneg m (S c) (S bs)))
-                    (mknonnegreal (fp_error m c (S bs)) (fp_error_nonneg m c (S bs)))
-                    (mknonnegreal (fp_error m c (S (S bs))) (fp_error_nonneg m c (S (S bs))))
-                   with
-                   "[$]").
-        * apply not_elem_of_dom_1; set_solver.
-        * intros i Hi.
-          apply elem_of_union in Hi as [?|Hs]; auto.
-          apply elem_of_singleton in Hs as ->.
-          auto.
-        * simpl.
+        rewrite fp_error_m_S /=.
+        lra.
+      + simpl.
+        iIntros (v) "(% & ? & [(% & ?) | (% &? )])".
+        * wp_pures.
+          wp_apply (wp_store_offset with "[$Ha]").
+          {
+            apply lookup_lt_is_Some_2.
+            rewrite HlenA //.
+          }
+          iIntros "Ha".
+          iApply "HK".
+          rewrite /is_bloom_filter_partial.
+          iExists hfuns', (ms_new ++ [(<[x:=v]> mcur)]), ms_old_tl, (<[v:=#true]> arr'),
+            ({[v]} ∪ idxs').
           rewrite size_union; [|set_solver].
           rewrite size_singleton.
-          rewrite fp_error_m_S -Hbs.
-          rewrite !S_INR.
-          rewrite plus_INR /=.
-          lra.
-        * iIntros (v2) "(%Hv2 & Hh2 & [(%HOut2 & Herr)|(%HIn2 & Herr )])".
-          ** wp_pures.
-             wp_apply (wp_store_offset with "[$Ha]").
-             {
-               apply lookup_lt_is_Some_2.
-               rewrite HlenA //.
-             }
+          simpl.
+          iFrame.
+          simpl.
+          iPureIntro.
+          repeat split.
+          ** rewrite -app_assoc //.
+          ** rewrite -app_assoc //.
+          ** rewrite insert_length //.
+          ** auto.
+          ** apply Forall_app_2; auto.
+             apply Forall_singleton.
+             set_solver.
+          ** intros e He.
+             specialize (Hidxs_old e He).
+             apply Forall_cons in Hidxs_old.
+             destruct Hidxs_old as [? Hidxs_old_tl].
+             apply (Forall_impl _ _ _ Hidxs_old_tl).
+             set_solver.
+          ** intros e He.
+             apply Forall_app; split.
+             *** specialize (Hidxs_new e He).
+                 apply (Forall_impl _ _ _ Hidxs_new).
+                 set_solver.
+             *** apply Forall_singleton.
+                 apply elem_of_union in He as [He|He].
+                 **** apply elem_of_singleton in He as ->.
+                      rewrite lookup_total_insert.
+                      set_solver.
+                 **** rewrite lookup_total_insert_ne; [|set_solver].
+                      specialize (Hidxs_old e He).
+                      apply Forall_cons in Hidxs_old.
+                      destruct Hidxs_old as [? ?].
+                      set_solver.
+          ** intros i Hi.
+             apply elem_of_union in Hi as [Hi|Hi].
+             *** apply elem_of_singleton in Hi as ->.
+                 rewrite list_lookup_insert //.
+                 real_solver.
+             *** rewrite list_lookup_insert_ne; auto.
+                 set_solver.
+          ** intros i Hi.
+             apply elem_of_union in Hi as [Hi|Hi]; auto.
+             apply elem_of_singleton in Hi as ->; done.
+          ** intros i Hleq Hi.
+             apply not_elem_of_union in Hi as [Hi1 Hi2].
+             apply not_elem_of_singleton in Hi1.
+             rewrite list_lookup_insert_ne; auto.
+
+        * wp_pures.
+          wp_apply (wp_store_offset with "[$Ha]").
+          {
+            apply lookup_lt_is_Some_2.
+            rewrite HlenA //.
+          }
+          iIntros "Ha".
+          iApply "HK".
+          rewrite /is_bloom_filter_partial.
+          iExists hfuns', (ms_new ++ [(<[x:=v]> mcur)]), ms_old_tl, (<[v:=#true]> arr'),
+            (idxs').
+          simpl.
+          iFrame.
+          simpl.
+          iPureIntro.
+          repeat split.
+          ** rewrite -app_assoc //.
+          ** rewrite -app_assoc //.
+          ** rewrite insert_length //.
+          ** auto.
+          ** apply Forall_app_2; auto.
+             apply Forall_singleton.
+             set_solver.
+          ** intros e He.
+             specialize (Hidxs_old e He).
+             apply Forall_cons in Hidxs_old.
+             destruct Hidxs_old as [? Hidxs_old_tl].
+             apply (Forall_impl _ _ _ Hidxs_old_tl).
+             set_solver.
+          ** intros e He.
+             apply Forall_app; split.
+             *** specialize (Hidxs_new e He).
+                 apply (Forall_impl _ _ _ Hidxs_new).
+                 set_solver.
+             *** apply Forall_singleton.
+                 apply elem_of_union in He as [He|He].
+                 **** apply elem_of_singleton in He as ->.
+                      rewrite lookup_total_insert.
+                      set_solver.
+                 **** rewrite lookup_total_insert_ne; [|set_solver].
+                      specialize (Hidxs_old e He).
+                      apply Forall_cons in Hidxs_old.
+                      destruct Hidxs_old as [? ?].
+                      set_solver.
+          ** intros i Hi.
+             destruct (decide (v = i)) as [-> | ?].
+             *** rewrite list_lookup_insert //.
+                 real_solver.
+             *** rewrite list_lookup_insert_ne //; auto.
+          ** intros i Hi; auto.
+          ** intros i Hleq Hi.
+             destruct (decide (v = i)) as [-> | ?].
+             *** rewrite list_lookup_insert //.
+             *** rewrite list_lookup_insert_ne //; auto.
+   - iModIntro.
+     iIntros "Hbf".
+     iApply "HΦ".
+     iPoseProof (bloom_filter_from_partial with "Hbf") as "Hbf".
+     replace ({[x]} ∪ s) with (s ∪ {[x]}) by set_solver.
+     iFrame.
+  Qed.
+
+
+  Lemma bloom_filter_lookup_spec (l : loc) (s : gset nat) (x rem : nat) :
+    {{{ is_bloom_filter l s (S rem) ∗ ⌜ x ∉ s ⌝
+    }}}
+      lookup_bloom_filter #l #x
+      {{{ v, RET v ; ⌜v = #false⌝ }}}.
+  Proof.
+    iIntros (Φ) "(Hbf & %Hx ) HΦ".
+    rewrite /lookup_bloom_filter /is_bloom_filter.
+    wp_pures.
+    iDestruct "Hbf" as (hfuns hs ms a arr idxs) "(Herr & Hl & %Hhfuns & %Hlenhs & Hhs & %HlenA & Ha & %Hms & %Hidxs & %Htrue & %Hbd & %Hfalse)".
+    wp_load.
+    wp_pures.
+    wp_alloc res as "Hres".
+    wp_pures.
+    iPoseProof (ec_weaken _ (fp_error 0 0 (size idxs)) with "Herr") as "Herr".
+    {
+      split.
+      - apply fp_error_nonneg.
+      - apply fp_error_weaken.
+    }
+    simpl.
+    wp_apply (wp_list_iter_invariant_HO
+             (λ l1 l2,
+               (∃ ms_old,
+                   ⌜ Forall (λ m : gmap nat nat, s = dom m) ms_old ⌝ ∗
+                   [∗ list] h;m ∈ l2;ms_old, hashfun filter_size h m) ∗
+               a ↦∗ arr ∗
+               ⌜ is_list_HO (l1 ++ l2) hfuns ⌝∗
+               ( res ↦ #false ∨
+                   (res ↦ #true ∗
+                    ↯ ((size idxs / (filter_size + 1)) ^ (length l2))%R)))%I
+           with "[][Ha Hhs Herr Hres]"); auto.
+    - iIntros (lpre w lsuf).
+      iIntros (Ψ).
+      iModIntro.
+      iIntros "((%ms_old & %Hms_old_dom & Hms_old_hf) & Ha & %Hhfuns' & [ Hr | (Hr & Herr)])".
+      + iIntros "HΨ".
+        wp_pures.
+        destruct ms_old as [| m ms_tail]; auto.
+        simpl.
+        iDestruct "Hms_old_hf" as "[Hmcur Hms_tail]".
+        wp_bind (w _).
+        wp_apply (wp_insert_basic _ _ _ m x with "Hmcur").
+        * apply not_elem_of_dom_1.
+          apply Forall_cons in Hms_old_dom as [-> ?].
+          done.
+        * iIntros (v) "(%Hv & Hhfw)".
+          wp_pures.
+          (destruct (decide (v ∈ idxs))).
+          ** wp_apply (wp_load_offset with "Ha"); [apply Htrue; auto|].
              iIntros "Ha".
              wp_pures.
-             wp_apply (wp_store_offset with "[$Ha]").
-             {
-               apply lookup_lt_is_Some_2.
-               rewrite insert_length HlenA //.
-             }
-             iIntros "Ha".
-             wp_pures.
-             simpl.
+             iApply "HΨ".
              iModIntro.
-             iApply "HΦ".
-             iExists 2.
-             iSplitR "Herr"; last first.
-             {
-               rewrite !Nat.add_succ_r Nat.add_0_r.
-               iFrame.
-             }
-             iExists h1, h2, (<[x:=v1]> m1), (<[x:=v2]> m2).
              iFrame.
-             iExists ((idxs ∪ {[v1]}) ∪ {[v2]}).
              iPureIntro.
-             repeat split.
-             *** rewrite !insert_length //.
-             *** set_solver.
-             *** set_solver.
-             *** intros e He.
-                 apply elem_of_union in He as [? | ?].
-                 **** apply Hidxs1 in H.
-                      admit.
-                 **** admit.
-             *** admit.
-             *** admit.
-             *** admit.
-             *** admit.
-             *** rewrite size_union; [|set_solver].
-                 rewrite size_union; [|set_solver].
-                 rewrite !size_singleton. real_solver.
- Admitted.
+             apply Forall_cons in Hms_old_dom as [??].
+             split; auto.
+             rewrite -app_assoc //.
+          ** wp_apply (wp_load_offset _ _ _ _ _ #false with "Ha"); [apply Hfalse; auto|].
+             iIntros "Ha".
+             wp_pures.
+             wp_store.
+             iApply "HΨ".
+             iModIntro.
+             iFrame.
+             iPureIntro.
+             apply Forall_cons in Hms_old_dom as [??].
+             split; auto.
+             rewrite -app_assoc //.
+      + iIntros "HΨ".
+        wp_pures.
+        destruct ms_old as [| m ms_tail]; auto.
+        iDestruct "Hms_old_hf" as "[Hmcur Hms_tail]".
+        wp_bind (w _).
+        assert
+          (forall z, (0 <= (size idxs / (filter_size + 1))^z)%R) as Haux.
+        {
+          intro z.
+          apply pow_le.
+          apply Rcomplements.Rdiv_le_0_compat; real_solver.
+        }
+        wp_apply (wp_insert_avoid_set_adv filter_size _ _ m _ idxs
+                    (mknonnegreal _ (Haux (length (w :: lsuf) )))
+                    (mknonnegreal _ (Haux (length lsuf )))
+                    0%NNR
+                        with "[$Herr $Hmcur]"); auto.
+        * apply Forall_cons in Hms_old_dom as [??].
+          apply not_elem_of_dom_1.
+          set_solver.
+        * simpl. lra.
+        * iIntros (v) "(%Hv & Hhfw & Herr)".
+          simpl.
+          iDestruct "Herr" as "[(%Hvout & Herr) | (%Hvin & Herr)]"; wp_pures.
+
+          ** wp_apply (wp_load_offset _ _ _ _ _ #false with "Ha"); [apply Hfalse; auto|].
+             iIntros "Ha".
+             wp_pures.
+             wp_store.
+             iApply "HΨ".
+             iModIntro.
+             iFrame.
+             iPureIntro.
+             apply Forall_cons in Hms_old_dom as [??].
+             split; auto.
+             rewrite -app_assoc //.
+
+          ** wp_apply (wp_load_offset with "Ha"); [apply Htrue; auto|].
+             iIntros "Ha".
+             wp_pures.
+             iApply "HΨ".
+             iModIntro.
+             iFrame.
+             repeat iSplit.
+             *** iPureIntro.
+                 apply Forall_cons in Hms_old_dom as [??]; auto.
+             *** iPureIntro.
+                 rewrite -app_assoc //.
+             *** iRight.
+                 iFrame.
+
+    - iFrame.
+      iSplit; auto.
+      iSplit; auto.
+      iSplit; auto.
+      iRight.
+      rewrite Hlenhs.
+      iFrame.
+    - iIntros "(?&?&?&[?|(?&Herr)])".
+      + wp_pures.
+        wp_load.
+        by iApply "HΦ".
+      + simpl.
+        iPoseProof (ec_contradict with "Herr") as "?"; done.
+ Qed.
 
 End bloom_filter.
